chore: add stepi cut theorems

Proofs/Experiments/Memcpy/MemCpyVCG.lean
@@ -7,9 +7,18 @@ Experimental: The goal is to prove that this program implements memcpy correctly
 using the VCG framework.
 -/
 import Arm
-import Tactics.StepThms
+import Tactics.CSE
+import Tactics.Rename
 import Tactics.Sym
+import Tactics.Rename
+import Tactics.Name
+import Tactics.ClearNamed
+import Tactics.StepThms
 import Correctness.ArmSpec
+import Arm.Insts.Common
+import Arm.Memory.SeparateAutomation
+import Arm.Syntax
+
 
 namespace Memcpy
 
@@ -36,6 +45,35 @@ def program : Program :=
      (0x8f4#64, 0x54ffff81#32),  /- b.ne 8e4 <mem_copy_loop> -/
      (0x8f8#64, 0xd65f03c0#32)   /- ret                      -/
     ]
+
+#genStepEqTheorems program
+
+open ArmStateNotation
+
+section PC
+
+/--# We define scoped notation for our cutpoint PCs to use in pattern matching. -/
+
+scoped notation "start" => 0x8e0#64
+scoped notation "loop_guard" => 0x8f4#64
+scoped notation "loop_post" => 0x8f8#64
+
+def pcs : List (BitVec 64) := [
+  start,
+  loop_guard,
+  loop_post
+  ]
+
+@[simp] theorem mem_pcs_iff (pc : BitVec 64) :
+    pc ∈ pcs ↔ pc = start ∨ pc = loop_guard ∨ pc = loop_post := by simp [pcs]
+
+@[simp] theorem start_mem_pcs : start ∈ pcs := by simp
+
+@[simp] theorem loop_guard_mem_pcs : loop_guard ∈ pcs := by simp
+
+@[simp] theorem loop_post_mem_pcs : loop_post ∈ pcs := by simp
+
+end PC
 
 
 /-- Precondition for the correctness of the MemCpy program. -/
@@ -129,9 +167,9 @@ def loop_inv (s0 si : ArmState) : Prop :=
 def assert (s0 si : ArmState) : Prop :=
   pre s0 ∧
   match (read_pc si) with
-  | 0x8e0#64 => -- First instruction
+  | start => -- First instruction
     si = s0
-  | 0x8f4#64 => -- Loop guard
+  | loop_guard => -- Loop guard
     loop_inv s0 si
   | 0x8f8 => -- Loop and program post
     post s0 si
@@ -150,6 +188,219 @@ instance : Spec' ArmState where
 -- #genStepEqThms program
 
 -------------------------------------------------------------------------------
+
+section CutTheorems
+
+--  /- 00000000000008e0 <mem_copy>:                         -/
+-- 1/7 (0x8e0#64, 0x14000004#32),  /- b   8f0 <loop_test>      -/
+--  /- 00000000000008e4 <mem_copy_loop>:                    -/
+-- 2/7 (0x8e4#64, 0x3cc10424#32),  /- ldr q4, [x1], #16        -/
+-- 3/7 (0x8e8#64, 0x3c810444#32),  /- str q4, [x2], #16        -/
+-- 4/7 (0x8ec#64, 0xd1000400#32),  /- sub x0, x0, #0x1         -/
+--  /- 00000000000008f0 <loop_test>:                        -/
+-- 5/7 (0x8f0#64, 0xf100001f#32),  /- cmp x0, #0x0             -/
+-- 6/7 (0x8f4#64, 0x54ffff81#32),  /- b.ne 8e4 <mem_copy_loop> -/
+-- 7/7 (0x8f8#64, 0xd65f03c0#32)   /- ret                      -/
+
+
+structure WellFormedAtPc (s : ArmState) (pc : BitVec 64) : Prop where
+  h_program : s.program = program
+  h_pc : r StateField.PC s = pc
+  h_err : r StateField.ERR s = StateError.None
+  h_sp_aligned : CheckSPAlignment s
+
+
+structure Stepped (s sn : ArmState) where
+  h_step : sn = stepi s
+
+abbrev Step_8e0_ef0 (s : ArmState) := WellFormedAtPc s 0x8e0
+
+--  /- 00000000000008e0 <mem_copy>:                         -/
+-- 1/7 (0x8e0#64, 0x14000004#32),  /- b   8f0 <loop_test>      -/
+theorem program.stepi_0x8e0_cut (s sn : ArmState)
+    (hs : Step_8e0_ef0 s)
+    (hstep : Stepped s sn) :
+    WellFormedAtPc sn 0x8f0 := by
+  obtain ⟨h_program, h_pc, h_err, h_sp_aligned⟩ := hs
+  have := program.stepi_eq_0x8e0 h_program h_pc h_err
+  obtain ⟨h_step⟩ := hstep
+  subst h_step
+  constructor <;> simp only [*, state_simp_rules, minimal_theory, bitvec_rules]
+
+/-
+  w StateField.PC 0x8e8#64
+    (w (StateField.GPR 0x1#5) (r (StateField.GPR 0x1#5) s + 0x10#64)
+      (w (StateField.SFP 0x4#5)
+        (BitVec.zeroExtend 128
+          (read_mem_bytes (8 <<< (BitVec.extractLsb 1 1 0x3#2 ++ 0x0#2).toNat / 8) (r (StateField.GPR 0x1#5) s) s))
+-/
+structure Step_8e4_8e8 (scur : ArmState) (snext : ArmState) extends WellFormedAtPc snext 0x8e8 : Prop where
+  h_x1 : snext.x1 = scur.x1 + 0x10#64
+  h_mem : snext.mem = scur.mem
+  h_q4 : snext.q4 = scur[scur.x1, 16]
+
+-- 2/7 (0x8e4#64, 0x3cc10424#32),  /- ldr q4, [x1], #16        -/
+theorem program.stepi_0x8e4_cut (scur snext : ArmState)
+    (hscur : WellFormedAtPc scur 0x8e4)
+    (hstep : Stepped scur snext) : Step_8e4_8e8 scur snext := by
+  obtain h_program := hscur.h_program
+  obtain h_pc := hscur.h_pc
+  obtain h_err := hscur.h_err
+  obtain h_sp_aligned := hscur.h_sp_aligned
+
+  have := program.stepi_eq_0x8e4 h_program h_pc h_err
+  simp [BitVec.extractLsb] at this
+  obtain ⟨h_step⟩ := hstep
+  subst h_step
+  constructor <;>  simp only [*, state_simp_rules, minimal_theory, bitvec_rules]
+  · constructor <;> simp? [*, state_simp_rules, minimal_theory, BitVec.extractLsb]
+
+-- 3/7 (0x8e8#64, 0x3c810444#32),  /- str q4, [x2], #16        -/
+structure Step_8e8_8ec (scur : ArmState) (snext : ArmState) extends WellFormedAtPc snext 0x8ec : Prop where
+  h_x2 : snext.x2 = scur.x2 + 0x10#64
+  h_mem : snext.mem = scur.mem.write_bytes 16 scur.x0 scur.q4
+
+theorem program.stepi_0x8e8_cut (sprev scur snext : ArmState)
+    (hs : Step_8e4_8e8 sprev scur)
+    (hstep : Stepped scur snext) : Step_8e8_8ec scur snext := by
+  obtain h_program := hs.h_program
+  obtain h_pc := hs.h_pc
+  obtain h_err := hs.h_err
+  obtain h_sp_aligned := hs.h_sp_aligned
+
+  have := program.stepi_eq_0x8e8 h_program h_pc h_err
+  simp [BitVec.extractLsb] at this
+  obtain ⟨h_step⟩ := hstep
+  subst h_step
+  constructor
+  · constructor <;> simp [*, state_simp_rules, minimal_theory, bitvec_rules]
+  · simp? [*, state_simp_rules, minimal_theory, BitVec.extractLsb]
+
+-- 4/7 (0x8ec#64, 0xd1000400#32),  /- sub x0, x0, #0x1         -/
+structure Step_8ec_8f0 (scur : ArmState) (snext : ArmState) extends WellFormedAtPc snext 0x8f0 : Prop where
+  h_x0 : snext.x0 = scur.x0 - 0x1#64
+  h_mem : snext.mem = scur.mem
+
+theorem program.stepi_0x8ec_cut (sprev scur snext : ArmState)
+    (hs : Step_8e8_8ec sprev scur)
+    (hstep : Stepped scur snext) : Step_8ec_8f0 scur snext := by
+  obtain h_program := hs.h_program
+  obtain h_pc := hs.h_pc
+  obtain h_err := hs.h_err
+  obtain h_sp_aligned := hs.h_sp_aligned
+
+  have := program.stepi_eq_0x8ec h_program h_pc h_err
+  simp [BitVec.extractLsb] at this
+  obtain ⟨h_step⟩ := hstep
+  subst h_step
+  constructor
+  · constructor <;> simp [*, state_simp_rules, minimal_theory, bitvec_rules]
+  · simp? (config := { ground := true, decide := true}) [*,
+      state_simp_rules, minimal_theory, BitVec.extractLsb, fst_AddWithCarry_eq_sub_neg]
+
+-- 5/7 (0x8f0#64, 0xf100001f#32),  /- cmp x0, #0x0             -/
+structure Step_8f0_8f4 (scur : ArmState) (snext : ArmState) extends WellFormedAtPc snext 0x8f4 : Prop where
+  h_mem : snext.mem = scur.mem
+  h_v : snext.V = (AddWithCarry scur.x0 0xffffffffffffffff#64 0x1#1).snd.v
+  h_c : snext.C = (AddWithCarry scur.x0 0xffffffffffffffff#64 0x1#1).snd.c
+  h_z : snext.Z = (AddWithCarry scur.x0 0xffffffffffffffff#64 0x1#1).snd.z
+  h_n : snext.N = (AddWithCarry scur.x0 0xffffffffffffffff#64 0x1#1).snd.n
+
+
+theorem program.stepi_0x8f0_cut (sprev scur snext : ArmState)
+    (hs : Step_8ec_8f0 sprev scur)
+    (hstep : Stepped scur snext) : Step_8f0_8f4 scur snext := by
+  obtain h_program := hs.h_program
+  obtain h_pc := hs.h_pc
+  obtain h_err := hs.h_err
+  obtain h_sp_aligned := hs.h_sp_aligned
+
+  have := program.stepi_eq_0x8f0 h_program h_pc h_err
+  simp (config := { ground := true, decide := true}) [BitVec.extractLsb,
+    fst_AddWithCarry_eq_sub_neg,
+    fst_AddWithCarry_eq_add] at this
+  obtain ⟨h_step⟩ := hstep
+  subst h_step
+  constructor
+  · constructor <;> simp [*, state_simp_rules, minimal_theory, bitvec_rules]
+  · simp? (config := { ground := true, decide := true}) [*,
+      state_simp_rules, minimal_theory, BitVec.extractLsb, fst_AddWithCarry_eq_sub_neg]
+
+-- 6/7 (0x8f4#64, 0x54ffff81#32),  /- b.ne 8e4 <mem_copy_loop> -/
+structure Step_8f4_8e4 (scur : ArmState) (snext : ArmState) extends WellFormedAtPc snext 0x8e4 : Prop where
+  h_mem : snext.mem = scur.mem
+  -- h_pc : snext.pc = 0x8e4#64
+
+theorem program.stepi_0x8f4_0x834_cut (sprev scur snext : ArmState)
+    (hs : Step_8f0_8f4 sprev scur)
+    (h_z : (r (StateField.FLAG PFlag.Z) scur) = 0#1)
+    (hstep : Stepped scur snext) : Step_8f4_8e4 scur snext := by
+  obtain h_program := hs.h_program
+  obtain h_pc := hs.h_pc
+  obtain h_err := hs.h_err
+  obtain h_sp_aligned := hs.h_sp_aligned
+
+  have := program.stepi_eq_0x8f4 h_program h_pc h_err
+  simp (config := { ground := true, decide := true}) [BitVec.extractLsb,
+    fst_AddWithCarry_eq_sub_neg,
+    fst_AddWithCarry_eq_add] at this
+  obtain ⟨h_step⟩ := hstep
+  subst h_step
+  constructor
+  · constructor <;> simp [*, state_simp_rules, minimal_theory, bitvec_rules]
+  · simp? (config := { ground := true, decide := true}) [*,
+      state_simp_rules, minimal_theory, BitVec.extractLsb, fst_AddWithCarry_eq_sub_neg]
+
+-- 6/7 (0x8f4#64, 0x54ffff81#32),  /- b.ne 8e4 <mem_copy_loop> -/
+structure Step_8f4_8f8 (scur : ArmState) (snext : ArmState) extends WellFormedAtPc snext 0x8f8 : Prop where
+  h_mem : snext.mem = scur.mem
+  -- h_pc : snext.pc = 0x8e4#64
+
+theorem program.stepi_0x8f4_0x8f8_cut (sprev scur snext : ArmState)
+    (hs : Step_8f0_8f4 sprev scur)
+    (h_z : (r (StateField.FLAG PFlag.Z) scur) = 1#1)
+    (hstep : Stepped scur snext) : Step_8f4_8f8 scur snext := by
+  obtain h_program := hs.h_program
+  obtain h_pc := hs.h_pc
+  obtain h_err := hs.h_err
+  obtain h_sp_aligned := hs.h_sp_aligned
+
+  have := program.stepi_eq_0x8f4 h_program h_pc h_err
+  simp (config := { ground := true, decide := true}) [BitVec.extractLsb,
+    fst_AddWithCarry_eq_sub_neg,
+    fst_AddWithCarry_eq_add] at this
+  obtain ⟨h_step⟩ := hstep
+  subst h_step
+  constructor
+  · constructor <;> simp [*, state_simp_rules, minimal_theory, bitvec_rules]
+  · simp? (config := { ground := true, decide := true}) [*,
+      state_simp_rules, minimal_theory, BitVec.extractLsb, fst_AddWithCarry_eq_sub_neg]
+
+
+-- 7/7 (0x8f8#64, 0xd65f03c0#32)   /- ret                      -/
+structure Step_8f8_ret (scur : ArmState) (snext : ArmState) : Prop where
+  h_mem : snext.mem = scur.mem
+
+theorem program.stepi_0x8f8_cut (sprev scur snext : ArmState)
+    (hs : Step_8f4_8f8 sprev scur)
+    (hstep : Stepped scur snext) : Step_8f8_ret scur snext := by
+  obtain h_program := hs.h_program
+  obtain h_pc := hs.h_pc
+  obtain h_err := hs.h_err
+  obtain h_sp_aligned := hs.h_sp_aligned
+
+  have := program.stepi_eq_0x8f8 h_program h_pc h_err
+  simp (config := { ground := true, decide := true}) [BitVec.extractLsb,
+    fst_AddWithCarry_eq_sub_neg,
+    fst_AddWithCarry_eq_add] at this
+
+  obtain ⟨h_step⟩ := hstep
+  subst h_step
+  constructor
+  · simp? (config := { ground := true, decide := true}) [*,
+      state_simp_rules, minimal_theory, BitVec.extractLsb, fst_AddWithCarry_eq_sub_neg]
+
+end CutTheorems
 
 theorem partial_correctness :
   PartialCorrectness ArmState := by
